Prove termination guarantees for interpreter.

src/heaplang/interpreter.v
@@ -5,12 +5,12 @@ From iris.itree Require Import wpi ub itree choice state later handler void inte
 From iris.itree.threadpool Require Import handler interleaving scheduler.
 From iris.itree.heaplang Require Import lang adequacy.
 
-Definition heaplang_ifn {R} (σ : state) (n : option nat) (t : itree heaplangE R) :
+Definition heaplang_ifn {R} (σ : state) (later_fuel : option nat) (t : itree heaplangE R) :
   itree voidE ((state * (R + last_thread_killed)) + later_exhausted + ub_crash) :=
-  ub_ifn (insert_voidE (later_ifn n (state_ifn σ (demonic_ifn (threadpool_ifn t))))).
+  ub_ifn (insert_voidE (later_ifn later_fuel (state_ifn σ (demonic_ifn (threadpool_ifn t))))).
 
-Lemma heaplang_ifn_irel {R} (t : itree heaplangE R) (σ : state) (n : option nat) :
-  heaplang_irel σ n t (heaplang_ifn σ n t).
+Lemma heaplang_ifn_irel {R} (t : itree heaplangE R) (σ : state) (later_fuel : option nat) :
+  heaplang_irel σ later_fuel t (heaplang_ifn σ later_fuel t).
 Proof.
   eexists. eexists. eexists.
   split; first apply threadpool_ifn_irel.
@@ -21,37 +21,37 @@ Qed.
 
 Variant timeout := Timeout.
 
-Definition heaplang_eval_itree σ n e :=
-  heaplang_ifn σ (Some n) (v ← compile_expr e ; yield_if_not_val e ;; Ret v).
+Definition heaplang_eval_itree σ later_fuel e :=
+  heaplang_ifn σ later_fuel (v ← compile_expr e ; yield_if_not_val e ;; Ret v).
 
-Definition heaplang_interpreter σ (n : nat) (e : expr) : (state * (val + last_thread_killed)) + ub_crash + timeout :=
-  match exec n (heaplang_eval_itree σ n e) with
+Definition heaplang_interpreter σ (fuel : nat) (later_fuel : option nat) (e : expr) : (state * (val + last_thread_killed)) + later_exhausted + ub_crash + timeout :=
+  match exec fuel (heaplang_eval_itree σ later_fuel e) with
   | None => inr Timeout
-  | Some (inl (inr LaterExhausted)) => inr Timeout
-  | Some (inl (inl r)) => inl (inl r)
-  | Some (inr UbCrash) => inl (inr UbCrash)
+  | Some x => inl x
   end.
 
-Lemma heaplang_interpreter_adequacy `{!invGS Σ} `{!heaplangHGS Σ} m e σ n Φ :
+Lemma heaplang_interpreter_adequacy `{!invGS Σ} `{!heaplangHGS Σ} m e σ fuel later_fuel Φ :
+  (m = Later → is_Some later_fuel) →
   state_interp σ -∗
-  £ n -∗
+  £ (default 0 later_fuel) -∗
   heap_inv -∗
   WP e @ m; ⊤ {{ Φ }} -∗
   |={⊤, ∅}=>
-    match heaplang_interpreter σ n e with
+    match heaplang_interpreter σ fuel later_fuel e with
     | inr Timeout => True
     | inl (inr UbCrash) => False
-    | inl (inl (σ, r)) => state_interp σ ∗
+    | inl (inl (inr LaterExhausted)) => ⌜is_Some later_fuel⌝
+    | inl (inl (inl (σ, r))) => state_interp σ ∗
         match r with | inl v => Φ v | inr LastThreadKilled => True end
     end.
 Proof.
-  iIntros "Hstate Hlc Hinv Hwp".
-  iDestruct (heaplang_adequacy_eval e σ (heaplang_eval_itree σ n e) with "Hstate [Hlc] Hinv Hwp") as "Heval".
+  iIntros (Hlat) "Hstate Hlc Hinv Hwp".
+  iDestruct (heaplang_adequacy_eval e σ (heaplang_eval_itree σ later_fuel e) with "Hstate [Hlc] Hinv Hwp") as "Heval".
   { apply heaplang_ifn_irel. }
   { eauto. }
   { done. }
   iMod "Heval" as "[%v [%Heval HΦ]]".
-  rewrite /heaplang_interpreter. destruct (exec n (heaplang_eval_itree σ n e)) eqn:Heq.
+  rewrite /heaplang_interpreter. destruct (exec fuel (heaplang_eval_itree σ later_fuel e)) eqn:Heq.
   * apply exec_eutt with (t' := (Ret v)) in Heq as [n' Heq]; last done.
     destruct n'; first done. injection Heq as <-.
     destruct v.
@@ -62,23 +62,40 @@ Proof.
   * destruct v; eauto.
 Qed.
 
-Lemma heaplang_interpreter_soundness `{!invGpreS Σ} `{!heaplangHGpreS Σ} m e σ n φ :
-  (∀ `{!invGS Σ} `{!heaplangHGS Σ}, ⊢ WP e @ m; ⊤ {{ v, ⌜φ v⌝ }}) →
-  match heaplang_interpreter σ n e with
-  | inr Timeout => True
-  | inl (inr UbCrash) => False
-  | inl (inl (_, inl v)) => φ v
-  | inl (inl (_, inr LastThreadKilled)) => True
+Lemma heaplang_interpreter_adequacy_termination `{!invGS Σ} `{!heaplangHGS Σ} e σ Φ :
+  state_interp σ -∗
+  heap_inv -∗
+  WP e @ Identity; ⊤ {{ Φ }} -∗
+  |={⊤, ∅}=>
+    ⌜∃ n, ∀ fuel, fuel ≥ n →
+      match heaplang_interpreter σ fuel None e with
+      | inr Timeout => False
+      | inl _ => True
+      end⌝.
+Proof.
+  iIntros "Hstate Hinv Hwp".
+  iMod lc_zero as "Hlc".
+  iDestruct (heaplang_adequacy_eval e σ (heaplang_eval_itree σ None e) with "Hstate [Hlc] Hinv Hwp") as "Heval".
+  { apply heaplang_ifn_irel. }
+  { intros. discriminate. }
+  { done. }
+  iMod "Heval" as "[%v [%Heval HΦ]]".
+  symmetry in Heval. apply exec_eutt with (r := v) (n := 1) in Heval as [fuel Heq]; last done.
+  iModIntro. iExists fuel. iIntros (fuel' Hlt).
+  rewrite /heaplang_interpreter (exec_stable fuel' fuel) // Heq //.
+Qed.
+
+Lemma heaplang_interpreter_soundness_termination `{!invGpreS Σ} `{!heaplangHGpreS Σ} e σ φ :
+  (∀ `{!invGS Σ} `{!heaplangHGS Σ}, ⊢ WP e @ Identity; ⊤ {{ v, ⌜φ v⌝ }}) →
+  ∃ n, ∀ fuel, fuel ≥ n → match heaplang_interpreter σ fuel None e with
+  | inr Timeout => False
+  | inl _ => True
   end.
 Proof.
-  intros Hwp. apply: (heaplang_soundness n).
+  intros Hwp. apply: (heaplang_soundness 0).
   iIntros (? ?) "#Hinv Hstate Hlc".
   iDestruct Hwp as "Hwp".
-  iDestruct (heaplang_interpreter_adequacy m e σ n with "Hstate Hlc Hinv Hwp") as "Hφ".
-  iMod "Hφ". iModIntro.
-  iApply step_fupdN_intro; first done. iModIntro.
-  destruct (heaplang_interpreter σ n e) as [[[σ' [v|[]]]|[]]|[]]; eauto.
-  iDestruct "Hφ" as "[_ $]".
+  by iDestruct (heaplang_interpreter_adequacy_termination e σ with "Hstate Hinv Hwp") as "Hφ".
 Qed.
 
 From iris.heap_lang Require Import proofmode notation.
